systems/chord-util/ChannelLemmas.v
@@ -264,8 +264,6 @@ Proof.
            simpl. repeat rewrite app_length. simpl. intuition.
         -- unfold label_input in *. congruence.
         -- unfold label_output in *. congruence.
-      * intuition.
-        find_apply_lem_hyp clients_not_in_failed; intuition.
       * apply in_channel_in_msgs; repeat find_rewrite; in_crush.
   - destruct ex. simpl.
     inv_prop lb_execution.
@@ -463,12 +461,14 @@ USED: In phase two.
   assert (exists st__dst, sigma gst' dst = Some st__dst)
     by eauto with invar.
   break_exists_name st__dst'.
-  assert (query_message_ok src dst (cur_request st__src) (delayed_queries st__dst)
+  assert (query_message_ok' src dst (cur_request st__src) (delayed_queries st__dst)
+                           (failed_nodes gst)
                            (channel gst src dst) (channel gst dst src))
-    by (eapply query_message_ok_invariant; eauto).
-  assert (query_message_ok src dst (cur_request st__src') (delayed_queries st__dst')
+    by (eapply query_message_ok'_invariant; eauto).
+  assert (query_message_ok' src dst (cur_request st__src') (delayed_queries st__dst')
+                           (failed_nodes gst')
                            (channel gst' src dst) (channel gst' dst src))
-    by (eapply query_message_ok_invariant; eauto with invar).
+    by (eapply query_message_ok'_invariant; eauto with invar).
   inv_prop open_request_to; expand_def.
   assert (cur_request_timeouts_ok' (cur_request st__src) (timeouts gst src))
     by eauto.
@@ -580,52 +580,57 @@ USED: In phase two.
           find_injection; tauto.
     }
     break_exists_name stm.
-    assert (query_message_ok src m__src (cur_request st__src) (delayed_queries stm)
+    assert (query_message_ok' src m__src (cur_request st__src) (delayed_queries stm)
+                             (failed_nodes gst)
                              (channel gst src m__src) (channel gst m__src src))
-      by (eapply query_message_ok_invariant; eauto).
+      by (eapply query_message_ok'_invariant; eauto).
     destruct (addr_eq_dec m__dst src); repeat find_rewrite.
     + subst.
       find_injection.
-      inv H11; repeat find_rewrite; find_injection;
-        try congruence;
-        try (exfalso; eapply_prop no_responses; eauto).
-      repeat find_rewrite; find_injection.
-      assert (res1 = res0); subst.
-      {
-        repeat find_apply_lem_hyp in_split; break_exists.
-        assert (no_responses (x0 ++ x2)) by eauto.
-        assert (~ In res0 x0)
-          by (intro; eapply_prop no_responses; [in_crush|]; eauto).
-        assert (~ In res0 x2)
-          by (intro; eapply_prop no_responses; [in_crush|]; eauto).
-        assert (In res0 (x11 ++ res0 :: x12)) by in_crush.
-        repeat find_rewrite.
-        in_crush.
-      }
-      destruct (response_payload_dec p).
-      * inv_prop query_message_ok;
-          try solve [exfalso; eapply_prop no_responses; eauto;
-                     eapply in_msgs_in_channel; find_rewrite; in_crush].
-        repeat find_rewrite; find_injection.
-        assert (res0 = p).
+      inv H11; try inv_prop query_message_ok;
+        repeat find_rewrite; find_injection;
+          try congruence;
+          try (exfalso; eapply_prop no_responses; eauto).
+      * admit.
+      * repeat find_rewrite; find_injection.
+        assert (res1 = res0); subst.
         {
-          assert (In p (channel gst (addr_of x1) src))
-            by (eapply in_msgs_in_channel; find_rewrite; in_crush).
           repeat find_apply_lem_hyp in_split; break_exists.
+          assert (no_responses (x0 ++ x2)) by eauto.
+          assert (~ In res0 x0)
+            by (intro; eapply_prop no_responses; [in_crush|]; eauto).
+          assert (~ In res0 x2)
+            by (intro; eapply_prop no_responses; [in_crush|]; eauto).
+          assert (In res0 (x13 ++ res0 :: x14)) by in_crush.
           repeat find_rewrite.
-          assert (no_responses (x5 ++ x6)) by eauto.
-          assert (~ In p x5)
-            by (intro; eapply_prop no_responses; [in_crush|]; eauto).
-          assert (~ In p x6)
-            by (intro; eapply_prop no_responses; [in_crush|]; eauto).
-          assert (In p (x0 ++ p :: x2)) by in_crush.
-          assert (In p (x5 ++ res0 :: x6)) by congruence.
           in_crush.
         }
-        subst; left; auto.
-      * assert (p <> res0) by (intro; subst; eauto).
+        destruct (response_payload_dec p).
+        -- inv_prop query_message_ok';
+             try inv_prop query_message_ok;
+             try solve [exfalso; eapply_prop no_responses; eauto;
+                        eapply in_msgs_in_channel; find_rewrite; in_crush].
+           admit.
+           repeat find_rewrite || find_injection.
+           assert (res0 = p).
+           {
+             assert (In p (channel gst (addr_of x1) src)).
+             eapply in_msgs_in_channel; find_rewrite; in_crush.
+             repeat find_apply_lem_hyp in_split; break_exists.
+             repeat find_rewrite.
+             assert (no_responses (x7 ++ x8)) by eauto.
+             assert (~ In p x7)
+               by (intro; eapply_prop no_responses; [in_crush|]; eauto).
+             assert (~ In p x8)
+               by (intro; eapply_prop no_responses; [in_crush|]; eauto).
+             assert (In p (x0 ++ p :: x2)) by in_crush.
+             assert (In p (x7 ++ res0 :: x8)) by congruence.
+             in_crush.
+           }
+           subst; eauto.
+      -- assert (p <> res0) by (intro; subst; eauto).
         right; split.
-        -- assert (~ query_response x p).
+        ++ assert (~ query_response x p).
            {
              intro; find_eapply_prop response_payload.
              inv_prop query_response; constructor.
@@ -637,7 +642,7 @@ USED: In phase two.
            apply in_or_app; right; eauto using in_remove_all_preserve.
            find_copy_eapply_lem_hyp recv_msg_not_right_response_preserves_cur_request; eauto.
            congruence.
-        -- apply in_msgs_in_channel; repeat find_apply_lem_hyp in_channel_in_msgs.
+        ++ apply in_msgs_in_channel; repeat find_apply_lem_hyp in_channel_in_msgs.
            apply in_or_app; right.
            repeat find_rewrite.
            simpl; in_crush; congruence.
@@ -660,4 +665,4 @@ USED: In phase two.
        apply in_msgs_in_channel; simpl;
          in_crush.
        find_eapply_lem_hyp clients_not_in_failed; eauto. intuition.
-Qed.
+Admitted.
